\chapter{Propiedades reales}

\section{Identidades pitagóricas}

\begin{gather*}
    \sin^2{(x)} + \cos^2{(x)} = 1
    \\
    \sec^2{(x)} - \tan^2{(x)} = 1
    \\
    \csc^2{(x)} - \cot^2{(x)} = 1
\end{gather*}


\section{Relaciones trigonométricas}

\begin{gather*}
    \sin{(x)}=\frac{O}{H}
    \\[1ex]
    \cos{(x)}=\frac{A}{H}
    \\[1ex]
    \tan{(x)}=\frac{O}{A}
    \\[1ex]
    \cot{(x)}=\frac{A}{O}
    \\[1ex]
    \sec{(x)}=\frac{H}{A}
    \\[1ex]
    \csc{(x)}=\frac{H}{O}
\end{gather*}


\section{Funciones trigonométricas}

\begin{gather*}
    \sin{(x)}=\frac{1}{\csc{(x)}}
    \\[1ex]
    \cos{(x)}=\dfrac{1}{\sec{(x)}}
    \\[1ex]
    \tan{(x)}=\frac{\sin{(x)}}{\cos{(x)}}
    \\[1ex]
    \cot{(x)}=\frac{\cos{(x)}}{\sin{(x)}}
    \\[1ex]
    \sec{(x)}=\frac{1}{\cos{(x)}}
    \\[1ex]
    \csc{(x)}=\frac{1}{\sin{(x)}}
\end{gather*}


\section{Ley de senos y cosenos}

\begin{equation*}
    \frac{A}{\sin{(\beta)}} = \frac{H}{\sin{(\gamma)}} = \frac{O}{\sin{(\alpha)}}
\end{equation*}

\begin{equation*}
    \left\{
    \begin{aligned}
        A^2 &= H^2+O^2-2HO.\cos{(A)}
        \\
        H^2 &= A^2+O^2-2AO.\cos{(H)}
        \\
        O^2 &= A^2+H^2-2AH.\cos{(O)}
    \end{aligned}
    \right.
\end{equation*}


\section{Suma y diferencia de ángulos}

\begin{equation*}
    \sin{(x \pm y)} = \sin{(x)} \, \cos{(y)} \pm \cos{(x)}\sin{(y)}
\end{equation*}

\begin{equation*}
    \cos{(x \pm y)} = \cos{(x)} \, \cos{(y)} \mp \sin{(x)}\sin{(y)}
\end{equation*}

\begin{equation*}
    \tan{(x \pm y)} = \dfrac{\tan{(x)} \pm \tan{(y)}}{1 \pm \tan{(x)} \, \tan{(y)}}
\end{equation*}

\begin{equation*}
    \cot{(x \pm y)} = \dfrac{\cot{(x)} \, \cot{(y)} \pm1}{\cot{(x)} \pm \cot{(y)}}
\end{equation*}

\begin{equation*}
    \sec{(x \pm y)} = \dfrac{1}{\cos{(x \pm y)}}
\end{equation*}

\begin{equation*}
    \csc{(x \pm y)} = \dfrac{1}{\sen{(x \pm y)}}
\end{equation*}


\section{Identidades de ángulo doble}

\begin{equation*}
    \sin{(2x)}=2 \, \sin{(x)} \, \cos{(x)}
\end{equation*}

\begin{equation*}
    \cos{(2x)}=\cos^2{(x)}-\sin^2{(x)}
\end{equation*}

\begin{equation*}
    \tan{(2x)}=\dfrac{2\tan{(x)}}{1-\tan^2{(x)}}
\end{equation*}

\begin{equation*}
    \cot{(2x)}=\dfrac{\cot^2{(x)}-1}{2\cot{(x)}}
\end{equation*}


\section{Propiedades logarítmicas}

\begin{equation*}
    \log_b{(x \, y)} = \log_b{(x)} + \log_b{(y)}
\end{equation*}

\begin{equation*}
    \log_b{\left( \frac{x}{y} \right)} = \log_b{(x)} - \log_b{(y)}
\end{equation*}

\begin{equation*}
    k \, \log_b{(x)} = \log_b{\left( x^k \right)}
\end{equation*}

\begin{equation*}
    \log_b{(x)}=\frac{\log_c{(x)}}{\log_c{(b)}}
\end{equation*}